Prove that 'collect' only collects reachable nodes.

Bdd/Basic.lean
@@ -1100,13 +1100,11 @@ lemma high_heap_eq_heap {O : OBdd n m} {h : O.1.root = node j} : (O.high h).1.he
 lemma oedge_of_low {h : O.1.root = node j} : OEdge O (O.low h) := ⟨rfl, edge_of_low (h := h)⟩
 lemma oedge_of_high {h : O.1.root = node j} : OEdge O (O.high h) := ⟨rfl, edge_of_high (h := h)⟩
 
-def OBdd.collect_helper (O : OBdd n m) : Vec Bool m × List (Fin m) → Vec Bool m × List (Fin m) := by
-  cases h : O.1.root with
-  | terminal b => exact id
+def OBdd.collect_helper (O : OBdd n m) : Vec Bool m × List (Fin m) → Vec Bool m × List (Fin m) :=
+  match h : O.1.root with
+  | terminal _ => id
   | node j =>
-    let v := O.1.heap[j].var
-    intro I
-    exact if I.1.get j then I else collect_helper (O.high h) (collect_helper (O.low h) ⟨I.1.set j true, j :: I.2⟩)
+    fun I ↦ if I.1.get j then I else collect_helper (O.high h) (collect_helper (O.low h) ⟨I.1.set j true, j :: I.2⟩)
 termination_by O
 decreasing_by
   exact oedge_of_high
@@ -1513,59 +1511,75 @@ theorem OBdd.collect_spec {O : OBdd n m} {j : Fin m} : Reachable O.1.heap O.1.ro
     intro i re1 re2
     exact List.Vector.get_replicate false i
 
-#eval example_bdd.collect
--- def OBdd.collect_helper (O : OBdd n m) : Vec Bool m × List (Fin m) → Vec Bool m × List (Fin m) := by
---   cases h : O.1.root with
---   | terminal b => exact id
---   | node j =>
---     let v := O.1.heap[j].var
---     intro I
---     exact if I.1.get j then I else collect_helper (O.high h) (collect_helper (O.low h) ⟨I.1.set j true, j :: I.2⟩)
--- termination_by O
--- decreasing_by
---   exact oedge_of_high
---   exact oedge_of_low
+theorem OBdd.collect_helper_spec_reverse (O : OBdd n m) (r : Pointer m) I :
+    Reachable O.1.heap r O.1.root →
+    (∀ i ∈ I.2, Reachable O.1.heap r (node i)) →
+    ∀ i ∈ (collect_helper O I).2, Reachable O.1.heap r (node i) := by
+  intro h0 h1 i h2
+  cases h : O.1.root with
+  | terminal b =>
+    rw [collect_helper_terminal' O h] at h2
+    exact h1 i h2
+  | node j =>
+    rw [collect_helper_node' O h] at h2
+    split at h2
+    next ht =>
+      exact h1 i h2
+    next hf =>
+      cases List.instDecidableMemOfLawfulBEq i (j :: I.2) with
+      | isTrue htt =>
+        cases htt with
+        | head as    => convert h0; symm; assumption
+        | tail b hin => exact h1 i hin
+      | isFalse hff =>
+        cases List.instDecidableMemOfLawfulBEq i ((O.low h).collect_helper (I.1.set j true, j :: I.2)).2 with
+        | isFalse hhf =>
+          rw [← high_heap_eq_heap (h := h)]
+          refine collect_helper_spec_reverse (O.high h) r _ ?_ ?_ i h2
+          · trans O.1.root
+            · exact h0
+            · exact reachable_of_edge (edge_of_high (h := h))
+          · intro i' hi'
+            simp only [high_heap_eq_heap]
+            rw [← low_heap_eq_heap (h := h)]
+            refine collect_helper_spec_reverse (O.low h) r _ ?_ ?_ i' hi'
+            · trans O.1.root
+              · exact h0
+              · exact reachable_of_edge (edge_of_low (h := h))
+            · intro i'' hi''
+              simp only at hi''
+              cases hi'' with
+              | head as     => simp only [low_heap_eq_heap]; convert h0; symm; assumption
+              | tail _ hi'' =>
+                simp only [low_heap_eq_heap]
+                exact h1 i'' hi''
+        | isTrue hht =>
+          rw [← low_heap_eq_heap (h := h)]
+          refine collect_helper_spec_reverse (O.low h) r _ ?_ ?_ i hht
+          · trans O.1.root
+            · exact h0
+            · exact reachable_of_edge (edge_of_low (h := h))
+          · intro i' hi'
+            simp only at hi'
+            cases hi' with
+            | head as    => simp only [low_heap_eq_heap]; convert h0; symm; assumption
+            | tail _ hi' =>
+              simp only [low_heap_eq_heap]
+              exact h1 i' hi'
+termination_by O
+decreasing_by
+  exact oedge_of_low
+  exact oedge_of_high
+  exact oedge_of_low
 
--- theorem OBdd.collect_helper_spec_reverse {O : OBdd n m} :
---     (∀ i ∈ I.2, Reachable O.1.heap O.1.root (node i)) →
---     ∀ i ∈ (collect_helper O I).2, Reachable O.1.heap O.1.root (node i) := by
---   intro h1 i h2
---   cases h : O.1.root with
---   | terminal b =>
---     rw [collect_helper_terminal' O h] at h2
---     rw [h] at h1
---     exact h1 i h2
---   | node j =>
---     rw [collect_helper_node' O h] at h2
---     split at h2
---     next ht =>
---       rw [h] at h1
---       exact h1 i h2
---     next hf =>
---       cases List.instDecidableMemOfLawfulBEq i (j :: I.2) with
---       | isTrue htt =>
---         cases htt with
---         | head as => left
---         | tail b hin =>
---           rw [h] at h1
---           exact h1 i hin
---       | isFalse hff =>
---         cases List.instDecidableMemOfLawfulBEq i ((O.low h).collect_helper (I.1.set j true, j :: I.2)).2 with
---         | isFalse hhf => sorry
---         | isTrue hht =>
---           rw [← h]
---           suffices s : (Reachable O.1.heap (O.low h).1.root (node i)) from Relation.ReflTransGen.trans (reachable_of_edge (edge_of_low (h := h) O.1)) s
---           rw [← low_heap_eq_heap (h := h)]
---           apply collect_helper_spec_reverse _ i hht
---           · intro i' hi'
---             simp only at hi'
---             sorry
+theorem OBdd.collect_spec_reverse {O : OBdd n m} {j : Fin m} : j ∈ collect O → Reachable O.1.heap O.1.root (node j) := by
+  intro h
+  simp only [collect] at h
+  apply collect_helper_spec_reverse O O.1.root (List.Vector.replicate m false, []) (Relation.ReflTransGen.refl)
+  · simp
+  · assumption
 
--- theorem OBdd.collect_spec_reverse {O : OBdd n m} {j : Fin m} : j ∈ collect O → Reachable O.1.heap O.1.root (node j) := by
---   intro h
---   simp only [collect] at h
---   unfold collect_helper at h
---   sorry
+theorem OBdd.mem_collect_iff_reachable {O : OBdd n m} {j : Fin m} : j ∈ collect O ↔ Reachable O.1.heap O.1.root (node j) := ⟨collect_spec_reverse, collect_spec⟩
 
 def OBdd.numPointers {n m} : OBdd n m → Nat := List.length ∘ collect
 
